Finiteness/Simplifications.lean
@@ -14,11 +14,11 @@ if it is `NonIncreasing`.
 
 @[simp]
 def simplify (f : RE α → RE α) : RE α → RE α
-  | l ⋒ r     => simplify f l ⋒ simplify f r
-  | ~r        => ~(simplify f r)
-  | l ⬝ r     => f (simplify f l ⬝ r)
-  | l ⋓ r     => f (simplify f l ⋓ simplify f r)
-  | r         => r
+  | l ⋒ r  => simplify f l ⋒ simplify f r
+  | ~r     => ~(simplify f r)
+  | l ⬝ r  => f (simplify f l ⬝ r)
+  | l ⋓ r  => f (simplify f l ⋓ simplify f r)
+  | r      => r
 
 -- define a type for nonincreasing fs
 @[simp]
@@ -30,7 +30,7 @@ theorem NonIncreasing_comp {f g : RE α → RE α} (ni_f : NonIncreasing f) (ni_
 theorem NonIncreasing_pieces [DecidableEq α] {r : RE α} (ni_f : NonIncreasing f) :
   pieces (simplify f r) ⊆[ (· ≅ ·) ] pieces r := fun re h =>
   match r with
-  | ε | Pred φ | ?=_ | ?!_ | ?<=_ | ?<!_ | _* => ⟨re,Rfl,h⟩
+  | ε | Pred φ | ?=_ | ?!_ | ?<=_ | ?<!_ | .Star _ => ⟨re,Rfl,h⟩
   | l ⬝ r  => by
     have := ni_f h
     simp only [simplify, pieces, mem_append, mem_map] at h this
@@ -39,7 +39,7 @@ theorem NonIncreasing_pieces [DecidableEq α] {r : RE α} (ni_f : NonIncreasing 
       have ⟨a1,a2,a3⟩ := toSumSubsets_monotone (NonIncreasing_pieces ni_f (r:=l)) _ g2
       subst g3
       exact ⟨a1 ⬝ r,Sim.Trans Rfl (CatCong a2),
-             by simp only [pieces, mem_append, mem_map, and_true, exists_eq_right]; exact Or.inl ⟨a1,a3,rfl⟩⟩
+             by simp only [pieces, mem_append, mem_map]; exact Or.inl ⟨a1,a3,rfl⟩⟩
     | Or.inr g1 => exact ⟨re,Rfl,by simp only [pieces, mem_append, mem_map]; exact Or.inr g1⟩
   | l ⋓ r  => by
     have := ni_f h
@@ -47,10 +47,10 @@ theorem NonIncreasing_pieces [DecidableEq α] {r : RE α} (ni_f : NonIncreasing 
     match this with
     | Or.inl g1 =>
       have ⟨a1,a2,a3⟩ := (NonIncreasing_pieces ni_f (r:=l)) _ g1
-      exact ⟨a1,Sim.Trans Rfl a2,by simp only [pieces, mem_append]; exact Or.inl a3⟩
+      exact ⟨a1,Sim.Trans Rfl a2,mem_append.mpr $ Or.inl a3⟩
     | Or.inr g1 =>
       have ⟨a1,a2,a3⟩ := (NonIncreasing_pieces ni_f (r:=r)) _ g1
-      exact ⟨a1,Sim.Trans Rfl a2,by simp only [pieces, mem_append]; exact Or.inr a3⟩
+      exact ⟨a1,Sim.Trans Rfl a2,mem_append.mpr $ Or.inr a3⟩
   | l ⋒ r  => by
     simp[pieces] at h
     let ⟨r1,r2,⟨hr1,hr2⟩,eq⟩ := h
@@ -58,8 +58,8 @@ theorem NonIncreasing_pieces [DecidableEq α] {r : RE α} (ni_f : NonIncreasing 
     have ⟨a1,a2,a3⟩ := toSumSubsets_monotone (NonIncreasing_pieces ni_f (r:=l)) _ hr1
     have ⟨b1,b2,b3⟩ := toSumSubsets_monotone (NonIncreasing_pieces ni_f (r:=r)) _ hr2
     exact ⟨a1 ⋒ b1,InterCong a2 b2,
-           by simp only [pieces, productWith, mem_map, Prod.exists, pair_mem_product,
-                         exists_eq_right_right, exists_eq_right]; exact ⟨a1,b1,⟨a3,b3⟩,rfl⟩⟩
+           by simp only [pieces, productWith, mem_map, Prod.exists, pair_mem_product];
+              exact ⟨a1,b1,⟨a3,b3⟩,rfl⟩⟩
   | ~r     => by
     simp[pieces] at h
     let ⟨r1,hr1,eq⟩ := h
@@ -104,40 +104,40 @@ def plus_not_bot [DecidableEq α] : RE α → RE α
 theorem plus_bot_l_ni [DecidableEq α] :
   NonIncreasing (α := α) plus_bot_l := fun r r1 h =>
   match r with
-  | ε | Pred ψ | ?=_ | ?!_ | ?<=_ | ?<!_ | _* | _⬝_ | _⋒_ | ~_ => h
+  | ε | Pred ψ | ?=_ | ?!_ | ?<=_ | ?<!_ | .Star _ | _⬝_ | _⋒_ | ~_ => h
   | l ⋓ r  =>
     match l with
     | Pred φ => by
       by_cases g : φ = ⊥
       . subst g; simp only [plus_bot_l] at h; exact mem_append.mpr (Or.inr h)
       . simp_all only [plus_bot_l, ↓reduceIte, pieces, cons_append, nil_append, mem_cons]
-    | ε | ?=_ | ?!_ | ?<=_ | ?<!_ | _* | _⬝_ | _⋒_ | _⋓_ | ~_ => h
+    | ε | ?=_ | ?!_ | ?<=_ | ?<!_ | .Star _ | _⬝_ | _⋒_ | _⋓_ | ~_ => h
 
 theorem plus_bot_r_ni [DecidableEq α] :
   NonIncreasing (α := α) plus_bot_r := fun r r1 h =>
   match r with
-  | ε | Pred ψ | ?=_ | ?!_ | ?<=_ | ?<!_ | _* | _⬝_ | _⋒_ | ~_  => h
+  | ε | Pred ψ | ?=_ | ?!_ | ?<=_ | ?<!_ | .Star _ | _⬝_ | _⋒_ | ~_  => h
   | l ⋓ r  =>
     match r with
     | Pred φ => by
       by_cases g : φ = ⊥
       . subst g; simp only [plus_bot_r] at h; exact mem_append.mpr (Or.inl h)
       . simp_all only [plus_bot_r, ↓reduceIte, pieces, mem_append, mem_cons, not_mem_nil, or_false]
-    | ε | ?=_ | ?!_ | ?<=_ | ?<!_ | _* | _⬝_ | _⋒_ | _⋓_ | ~_ => h
+    | ε | ?=_ | ?!_ | ?<=_ | ?<!_ | .Star _ | _⬝_ | _⋒_ | _⋓_ | ~_ => h
 
 theorem mult_eps_ni :
   NonIncreasing (α := α) mult_eps := fun r r1 h =>
   match r with
-  | ε | Pred ψ | ?=_ | ?!_ | ?<=_ | ?<!_ | _* | _⋒_ | _⋓_ | ~_ => h
+  | ε | Pred ψ | ?=_ | ?!_ | ?<=_ | ?<!_ | .Star _ | _⋒_ | _⋓_ | ~_ => h
   | l ⬝ r  =>
     match l with
     | ε      => by simp_all only [mult_eps, pieces, mem_append, mem_map, or_true]
-    | Pred ψ | ?=_ | ?!_ | ?<=_ | ?<!_ | _* | _⬝_ | _⋒_ | _⋓_ | ~_ => h
+    | Pred ψ | ?=_ | ?!_ | ?<=_ | ?<!_ | .Star _ | _⬝_ | _⋒_ | _⋓_ | ~_ => h
 
 theorem mult_bot_ni [DecidableEq α] :
   NonIncreasing (α := α) mult_bot := fun r r1 h =>
   match r with
-  | ε | Pred ψ | ?=_ | ?!_ | ?<=_ | ?<!_ | _* | _⋒_ | _⋓_ | ~_ => h
+  | ε | Pred ψ | ?=_ | ?!_ | ?<=_ | ?<!_ | .Star _ | _⋒_ | _⋓_ | ~_ => h
   | l ⬝ r  =>
     match r with
     | Pred ψ => by
@@ -145,12 +145,12 @@ theorem mult_bot_ni [DecidableEq α] :
       . subst g
         simp_all only [mult_bot, ↓reduceIte, pieces, mem_cons, not_mem_nil, or_false, mem_append, mem_map, or_true]
       . simp only [mult_bot, g] at h; exact h
-    | ε | ?=_ | ?!_ | ?<=_ | ?<!_ | _* | _⬝_ | _⋒_ | _⋓_ | ~_ => h
+    | ε | ?=_ | ?!_ | ?<=_ | ?<!_ | .Star _ | _⬝_ | _⋒_ | _⋓_ | ~_ => h
 
 theorem distr_ni :
   NonIncreasing (α := α) distr := fun r r1 h =>
   match r with
-  | ε | Pred ψ | ?=_ | ?!_ | ?<=_ | ?<!_ | _* | _⋒_ | _⋓_ | ~_ => h
+  | ε | Pred ψ | ?=_ | ?!_ | ?<=_ | ?<!_ | .Star _ | _⋒_ | _⋓_ | ~_ => h
   | (l ⋓ r) ⬝ g  => by
     simp[pieces] at h
     match h with
@@ -185,12 +185,12 @@ theorem distr_ni :
         | Or.inr g2 =>
           unfold pieces; simp only [mem_append, mem_map]
           exact Or.inr g2
-    | ε | Pred ψ | ?=_ | ?!_ | ?<=_ | ?<!_ | _* | _⬝_ | _⋒_ | ~_ => h
+    | ε | Pred ψ | ?=_ | ?!_ | ?<=_ | ?<!_ | .Star _ | _⬝_ | _⋒_ | ~_ => h
 
 theorem plus_not_bot_ni [DecidableEq α] :
   NonIncreasing (α := α) plus_not_bot := fun r r1 h =>
   match r with
-  | ε | Pred ψ | ?=_ | ?!_ | ?<=_ | ?<!_ | _* | _⋒_ | _⬝_ | ~_ => h
+  | ε | Pred ψ | ?=_ | ?!_ | ?<=_ | ?<!_ | .Star _ | _⋒_ | _⬝_ | ~_ => h
   | l ⋓ r =>
     match l with
     | ~l =>
@@ -199,8 +199,8 @@ theorem plus_not_bot_ni [DecidableEq α] :
         by_cases g : ψ = ⊥
         . subst g; simp only [plus_not_bot, ↓reduceIte] at h; exact mem_append.mpr $ Or.inl h
         . simp only [plus_not_bot, g, ↓reduceIte] at h; exact h
-      | ε | ?=_ | ?!_ | ?<=_ | ?<!_ | _* | _⬝_ | _⋒_ | _⋓_ | ~_ => h
-    | ε | Pred ψ | ?=_ | ?!_ | ?<=_ | ?<!_ | _* | _⬝_ | _⋒_ | _⋓_ => h
+      | ε | ?=_ | ?!_ | ?<=_ | ?<!_ | .Star _ | _⬝_ | _⋒_ | _⋓_ | ~_ => h
+    | ε | Pred ψ | ?=_ | ?!_ | ?<=_ | ?<!_ | .Star _ | _⬝_ | _⋒_ | _⋓_ => h
 
 -- define as a fold
 def NonIncreasing_simps [DecidableEq α] : RE α → RE α :=
@@ -262,19 +262,19 @@ def pieces' : RE α → List (RE α)
   | l ⋓ r     => pieces' l ++ pieces' r
   | l ⋒ r     => Pred ⊥ :: productWith (· ⋒ ·) ⊕(pieces' l) ⊕(pieces' r) ++ pieces' l ++ pieces' r
   | l ⬝ r     => map (· ⬝ r) ⊕(pieces' l) ++ pieces' r ++ pieces' l
-  | r *       => Pred ⊥ :: r* :: map (· ⬝ r*) ⊕(pieces' r) ++ pieces' r
+  | .Star r   => Pred ⊥ :: r* :: map (· ⬝ r*) ⊕(pieces' r) ++ pieces' r
   | ~ r       => Pred ⊥ :: map (~ ·) ⊕(pieces' r) ++ pieces' r
 
 theorem bot_in_pieces' {r : RE α} : Pred ⊥ ∈ pieces' r := by
   match r with
-  | ε | Pred ψ | ?=_ | ?!_ | ?<=_ | ?<!_ | ~r | l ⋒ r | r* => simp[pieces']
+  | ε | Pred ψ | ?=_ | ?!_ | ?<=_ | ?<!_ | ~r | l ⋒ r | .Star r => simp[pieces']
   | l ⋓ r => simp[pieces']; exact Or.inl bot_in_pieces'
   | l ⬝ r => simp[pieces']; exact Or.inl bot_in_pieces'
 
 theorem eps_in_pieces' {r : RE α} : ε ∈ pieces' r := by
   match r with
   | ε | Pred ψ | ?=_ | ?!_ | ?<=_ | ?<!_ => simp[pieces']
-  | r* | ~r => simp[pieces']; exact eps_in_pieces'
+  | .Star r | ~r => simp[pieces']; exact eps_in_pieces'
   | l ⬝ r | l ⋓ r | l ⋒ r => simp[pieces']; exact Or.inl eps_in_pieces'
 
 -- ⊥ ⬝ r → ⊥
@@ -319,12 +319,15 @@ def mult_eps_r : RE α → RE α
   | r ⬝ ε => r
   | r => r
 
-def nonincreasing' (f : RE α → RE α) := ∀ ⦃r⦄, pieces' (f r) ⊆ pieces' r
+def Nonincreasing' (f : RE α → RE α) := ∀ ⦃r⦄, pieces' (f r) ⊆ pieces' r
+
+theorem Nonincreasing'_comp {f g : RE α → RE α} (ni_f : Nonincreasing' f) (ni_g : Nonincreasing' g):
+  Nonincreasing' (g ∘ f) := fun _ _ h => ni_f (ni_g h)
 
 theorem mult_bot_l_ni [DecidableEq α] :
-  nonincreasing' (α := α) mult_bot_l := fun r r1 h =>
+  Nonincreasing' (α := α) mult_bot_l := fun r r1 h =>
   match r with
-  | ε | Pred ψ | ?=_ | ?!_ | ?<=_ | ?<!_ | _* | _⋒_ | _⋓_ | ~_ => h
+  | ε | Pred ψ | ?=_ | ?!_ | ?<=_ | ?<!_ | .Star _ | _⋒_ | _⋓_ | ~_ => h
   | l ⬝ r  =>
     match l with
     | Pred ψ => by
@@ -336,12 +339,12 @@ theorem mult_bot_l_ni [DecidableEq α] :
         | Or.inl h1 => subst h1; exact eps_in_pieces'
         | Or.inr h1 => subst h1; exact bot_in_pieces'
       . simp only [mult_bot_l, g] at h; exact h
-    | ε | ?=_ | ?!_ | ?<=_ | ?<!_ | _* | _⬝_ | _⋒_ | _⋓_ | ~_ => h
+    | ε | ?=_ | ?!_ | ?<=_ | ?<!_ | .Star _ | _⬝_ | _⋒_ | _⋓_ | ~_ => h
 
 theorem inter_bot_l_ni [DecidableEq α] :
-  nonincreasing' (α := α) inter_bot_l := fun r r1 h =>
+  Nonincreasing' (α := α) inter_bot_l := fun r r1 h =>
   match r with
-  | ε | Pred ψ | ?=_ | ?!_ | ?<=_ | ?<!_ | _* | _⬝_ | _⋓_ | ~_ => h
+  | ε | Pred ψ | ?=_ | ?!_ | ?<=_ | ?<!_ | .Star _ | _⬝_ | _⋓_ | ~_ => h
   | l ⋒ r  =>
     match l with
     | Pred ψ => by
@@ -353,12 +356,12 @@ theorem inter_bot_l_ni [DecidableEq α] :
           Prod.exists, pair_mem_product]
         exact Or.inr $ Or.inr $ Or.inl h
       . simp only [inter_bot_l, g] at h; exact h
-    | ε | ?=_ | ?!_ | ?<=_ | ?<!_ | _* | _⬝_ | _⋒_ | _⋓_ | ~_ => h
+    | ε | ?=_ | ?!_ | ?<=_ | ?<!_ | .Star _ | _⬝_ | _⋒_ | _⋓_ | ~_ => h
 
 theorem inter_bot_r_ni [DecidableEq α] :
-  nonincreasing' (α := α) inter_bot_r := fun r r1 h =>
+  Nonincreasing' (α := α) inter_bot_r := fun r r1 h =>
   match r with
-  | ε | Pred ψ | ?=_ | ?!_ | ?<=_ | ?<!_ | _* | _⬝_ | _⋓_ | ~_ => h
+  | ε | Pred ψ | ?=_ | ?!_ | ?<=_ | ?<!_ | .Star _ | _⬝_ | _⋓_ | ~_ => h
   | l ⋒ r  =>
     match r with
     | Pred ψ => by
@@ -369,12 +372,12 @@ theorem inter_bot_r_ni [DecidableEq α] :
           Prod.exists, pair_mem_product]
         exact Or.inr $ Or.inr $ Or.inr h
       . simp only [inter_bot_r, g] at h; exact h
-    | ε | ?=_ | ?!_ | ?<=_ | ?<!_ | _* | _⬝_ | _⋒_ | _⋓_ | ~_ => h
+    | ε | ?=_ | ?!_ | ?<=_ | ?<!_ | .Star _ | _⬝_ | _⋒_ | _⋓_ | ~_ => h
 
 theorem double_neg_ni [DecidableEq α] :
-  nonincreasing' (α := α) double_neg := fun r r1 h =>
+  Nonincreasing' (α := α) double_neg := fun r r1 h =>
   match r with
-  | ε | Pred ψ | ?=_ | ?!_ | ?<=_ | ?<!_ | _* | _⬝_ | _⋓_ | _⋒_  => h
+  | ε | Pred ψ | ?=_ | ?!_ | ?<=_ | ?<!_ | .Star _ | _⬝_ | _⋓_ | _⋒_  => h
   | ~r =>
     match r with
     | ~r => by
@@ -384,12 +387,12 @@ theorem double_neg_ni [DecidableEq α] :
       unfold pieces'
       simp only [cons_append, mem_cons, mem_append, mem_map]
       exact Or.inr $ Or.inr $ Or.inr $ Or.inr h
-    | ε | Pred ψ | ?=_ | ?!_ | ?<=_ | ?<!_ | _* | _⬝_ | _⋓_ | _⋒_  => h
+    | ε | Pred ψ | ?=_ | ?!_ | ?<=_ | ?<!_ | .Star _ | _⬝_ | _⋓_ | _⋒_  => h
 
 theorem inter_not_bot_r_ni [DecidableEq α] :
-  nonincreasing' (α := α) inter_not_bot_r := fun r r1 h =>
+  Nonincreasing' (α := α) inter_not_bot_r := fun r r1 h =>
   match r with
-  | ε | Pred ψ | ?=_ | ?!_ | ?<=_ | ?<!_ | _* | _⬝_ | _⋓_ | ~_  => h
+  | ε | Pred ψ | ?=_ | ?!_ | ?<=_ | ?<!_ | .Star _ | _⬝_ | _⋓_ | ~_  => h
   | l ⋒ r =>
     match r with
     | ~r =>
@@ -401,13 +404,13 @@ theorem inter_not_bot_r_ni [DecidableEq α] :
           simp only [productWith, cons_append, append_assoc, mem_cons, mem_append, mem_map, Prod.exists, pair_mem_product]
           exact Or.inr $ Or.inr $ Or.inl h
         . simp[g] at h; exact h
-      | ε | ?=_ | ?!_ | ?<=_ | ?<!_ | _* | _⬝_ | _⋓_ | _⋒_ | ~_ => h
-    | ε | Pred ψ | ?=_ | ?!_ | ?<=_ | ?<!_ | _* | _⬝_ | _⋓_ | _⋒_ => h
+      | ε | ?=_ | ?!_ | ?<=_ | ?<!_ | .Star _ | _⬝_ | _⋓_ | _⋒_ | ~_ => h
+    | ε | Pred ψ | ?=_ | ?!_ | ?<=_ | ?<!_ | .Star _ | _⬝_ | _⋓_ | _⋒_ => h
 
 theorem inter_not_bot_l_ni [DecidableEq α] :
-  nonincreasing' (α := α) inter_not_bot_l := fun r r1 h =>
+  Nonincreasing' (α := α) inter_not_bot_l := fun r r1 h =>
   match r with
-  | ε | Pred ψ | ?=_ | ?!_ | ?<=_ | ?<!_ | _* | _⬝_ | _⋓_ | ~_  => h
+  | ε | Pred ψ | ?=_ | ?!_ | ?<=_ | ?<!_ | .Star _ | _⬝_ | _⋓_ | ~_  => h
   | l ⋒ r =>
     match l with
     | ~r =>
@@ -419,23 +422,72 @@ theorem inter_not_bot_l_ni [DecidableEq α] :
           simp only [productWith, cons_append, append_assoc, mem_cons, mem_append, mem_map, Prod.exists, pair_mem_product]
           exact Or.inr $ Or.inr $ Or.inr h
         . simp only [inter_not_bot_l, g] at h; exact h
-      | ε | ?=_ | ?!_ | ?<=_ | ?<!_ | _* | _⬝_ | _⋓_ | _⋒_ | ~_ => h
-    | ε | Pred ψ | ?=_ | ?!_ | ?<=_ | ?<!_ | _* | _⬝_ | _⋓_ | _⋒_ => h
+      | ε | ?=_ | ?!_ | ?<=_ | ?<!_ | .Star _ | _⬝_ | _⋓_ | _⋒_ | ~_ => h
+    | ε | Pred ψ | ?=_ | ?!_ | ?<=_ | ?<!_ | .Star _ | _⬝_ | _⋓_ | _⋒_ => h
 
 theorem mult_eps_r_ni :
-  nonincreasing' (α := α) mult_eps_r := fun r r1 h =>
+  Nonincreasing' (α := α) mult_eps_r := fun r r1 h =>
   match r with
-  | ε | Pred ψ | ?=_ | ?!_ | ?<=_ | ?<!_ | _* | _⋒_ | _⋓_ | ~_ => h
+  | ε | Pred ψ | ?=_ | ?!_ | ?<=_ | ?<!_ | .Star _ | _⋒_ | _⋓_ | ~_ => h
   | l ⬝ r  =>
     match r with
     | ε      => by
       simp only [mult_eps_r] at h; unfold pieces'
       simp only [append_assoc, mem_append, mem_map]
       exact Or.inr $ Or.inr h
-    | Pred ψ | ?=_ | ?!_ | ?<=_ | ?<!_ | _* | _⬝_ | _⋒_ | _⋓_ | ~_ => h
+    | Pred ψ | ?=_ | ?!_ | ?<=_ | ?<!_ | .Star _ | _⬝_ | _⋒_ | _⋓_ | ~_ => h
 
 def NonIncreasing_simps' [DecidableEq α] : RE α → RE α :=
   mult_eps_r ∘ inter_not_bot_l ∘ inter_not_bot_r ∘ double_neg ∘ NonIncreasing_simps ∘ mult_bot_l ∘ inter_bot_l ∘ inter_bot_r
+
+-- theorem distr'_ni :
+--   Nonincreasing' (α := α) distr := fun r r1 h =>
+--   match r with
+--   | ε | Pred ψ | ?=_ | ?!_ | ?<=_ | ?<!_ | .Star _ | _⋒_ | _⋓_ | ~_ => h
+--   | (l ⋓ r) ⬝ g  => by
+--     simp[pieces'] at h
+--     match h with
+--     | Or.inl ⟨a1,a2,eq⟩ =>
+--       subst eq
+--       simp only [pieces', mem_append, mem_map, Concatenation.injEq, and_true, exists_eq_right]
+--       exact Or.inl (Or.inl (toSum_appendL a2))
+--     | Or.inr g' =>
+--       match g' with
+--       | Or.inl a1 => unfold pieces'; simp; exact Or.inr $ Or.inl a1
+--       | Or.inr g1 =>
+--         simp[pieces']
+--         match g1 with
+--         | Or.inl g2 => exact Or.inr $ Or.inr $ Or.inl g2
+--         | Or.inr g2 =>
+--           match g2 with
+--           | Or.inl ⟨a1,a2,eq⟩ => subst eq; exact Or.inl ⟨a1,toSum_appendR a2,rfl⟩
+--           | Or.inr g3 => exact Or.inr (by aesop)
+--   | l ⬝ g =>
+--     match l with
+--     | l1 ⋓ l2 => by
+--       simp only [distr, pieces', append_assoc, mem_append, mem_map] at h
+--       match h with
+--       | Or.inl ⟨a1,a2,a3⟩ =>
+--         subst a3
+--         simp only [pieces', mem_append, mem_map, Concatenation.injEq, and_true, exists_eq_right]
+--         exact Or.inl $ Or.inl (toSum_appendL a2)
+--       | Or.inr g1 =>
+--         match g1 with
+--         | Or.inl g2 =>
+--           unfold pieces'
+--           simp only [mem_append, mem_map]
+--           exact Or.inl $ Or.inr g2
+--         | Or.inr g2 =>
+--           simp only [pieces', mem_append, mem_map]
+--           sorry
+--     | ε | Pred ψ | ?=_ | ?!_ | ?<=_ | ?<!_ | .Star _ | _⬝_ | _⋒_ | ~_ => h
+
+-- def NonIncreasing_simps'_proof [DecidableEq α] :
+--   NonIncreasing (α := α) NonIncreasing_simps' := fun r _ h =>
+--   have step0 : Nonincreasing' (α:=α) (mult_eps_r ∘ inter_not_bot_l ∘ inter_not_bot_r ∘ double_neg ∘ NonIncreasing_simps' ∘ mult_bot_l ∘ inter_bot_l) :=
+--     Nonincreasing'_comp (Nonincreasing'_comp (Nonincreasing'_comp (Nonincreasing'_comp (Nonincreasing'_comp (Nonincreasing'_comp inter_bot_l_ni mult_bot_l_ni) sorry) double_neg_ni) inter_not_bot_r_ni) inter_not_bot_l_ni) mult_eps_r_ni
+--   have step := Nonincreasing'_comp (g:= mult_eps_r ∘ inter_not_bot_l ∘ inter_not_bot_r ∘ double_neg ∘ NonIncreasing_simps' ∘ mult_bot_l ∘ inter_bot_l ∘ inter_bot_r) (r:=r) distr'_ni step0
+--   step h
 
 def step_with_simp' [DecidableEq α] (r : RE α) : List (RE α) :=
   map (simplify NonIncreasing_simps') (step r)
@@ -444,3 +496,31 @@ def step_with_simp' [DecidableEq α] (r : RE α) : List (RE α) :=
 def steps_with_simp' [DecidableEq α] (r : RE α) : ℕ → List (RE α)
   | 0 => [r]
   | Nat.succ n => map step_with_simp' (steps_with_simp' r n) |> flatten
+
+-- theorem fin_step_with_simp' [DecidableEq α] {r : RE α} :
+--   step_with_simp' r ⊆[ (· ≅ ·) ] ⊕(pieces r) := fun e1 in_step => by
+--   simp only [step_with_simp', mem_map] at in_step
+--   let ⟨a1,a2,a3⟩ := in_step
+--   subst a3
+--   have ⟨p1,p2,p3⟩ := pieces_refl (r:=simplify NonIncreasing_simps' a1)
+--   have ⟨m1,m2,m3⟩ : toSum p1 ∈[ (· ≅ ·) ] ⊕((pieces (simplify NonIncreasing_simps' a1))) :=
+--     ⟨toSum p1, Rfl, by simp[toSumSubsets]; exact ⟨p1,p2,⟨p1,Perm.refl _,rfl⟩⟩⟩
+--   -- have inter_step := toSumSubsets_monotone $ NonIncreasing_pieces (r:=a1) sorry -- NonIncreasing_simps'_proof
+--   -- have ⟨o1,o2,o3⟩ := toSumSubsets_pieces_trans (inter_step _ m3) (step_to_toSumSubsets _ a2)
+--   -- exists o1; exists Sim.Trans (Sim.Trans (Sym p3) m2) o2
+--   sorry
+
+-- theorem finiteness_simp' [DecidableEq α] {r : RE α} :
+--   steps_with_simp' r n ⊆[ (· ≅ ·) ] ⊕(pieces r) := fun e1 h =>
+--   match n with
+--   | 0 => by
+--     simp only [steps_with_simp', mem_cons, not_mem_nil, or_false] at h
+--     subst h; exact toSumSubsets_pieces_refl
+--   | Nat.succ n => by
+--     simp at h
+--     let ⟨e2,e2_steps_n,e1_step_e2⟩ := h
+--     have ⟨q1,q1_eqv,ih⟩ := finiteness_simp' _ e2_steps_n
+--     have ⟨xs,xs_eqv,hxs⟩ := fin_step_with_simp' _ e1_step_e2
+--     have e2_in : e2 ∈[ (· ≅ ·) ] ⊕(pieces r) := ⟨q1,q1_eqv,ih⟩
+--     have e_in  : e1 ∈[ (· ≅ ·) ] ⊕(pieces e2) := ⟨xs,xs_eqv,hxs⟩
+--     exact toSumSubsets_pieces_trans e_in e2_in
